---
title: 1.1.1 Luminosity (Derivations)
parent: 1.1 Luminosity
nav_order: 1
layout: default
---

# Luminosity in Accelerator Physics (Derivations)

Derivations from Luminosity Page

## 1a. Luminosity of Round, Gaussian Beams

Starting from this definition of Luminosity:

$$ \mathcal{L} = KfN_1N_2N_b\int_{-\infty}^{\infty}\int_{-\infty}^{\infty}\int_{-\infty}^{\infty}\int_{-\infty}^{\infty} \rho_1(x, y, s, -s_0) \rho_2(x, y, s, s_0) dx dy ds ds_0$$

For a gaussian distribution for one beam:\
$$\rho_{iz}(z) = \frac{1}{\sqrt{2\pi}\sigma_{iz}}\exp(-\frac{z^2}{\sigma_{iz}}); i = 1,2; z = x, y$$\
$$\rho_{is}(s, s_0) = \frac{1}{\sqrt{2\pi}\sigma_{is}}\exp(-\frac{(s + s_0)^2}{\sigma_{is}}); i = 1,2$$

For two beams heading toward each other ($$v_1 = - v_2$$), then $$K = 2$$

And assumming a round beam:\
$$\sigma_{x1} = \sigma_{x2} = \sigma_{x}$$ = constant\
$$\sigma_{y1} = \sigma_{y2} = \sigma_{y}$$ = constant\
$$\sigma_{s1} = \sigma_{s2} = \sigma_{s}$$ = constant

Then:\
$$ \Rightarrow \rho_1\rho_2 = \frac{1}{(2\pi)^3(\sigma_x\sigma_y\sigma_z)^2}\exp(-(\frac{x}{\sigma_x})^2 + (\frac{y}{\sigma_y})^2 + \frac{(s + s_0)^2 + (s - s_0)^2}{2\sigma_z^2})$$\
$$= \frac{1}{(2\pi)^3(\sigma_x\sigma_y\sigma_z)^2}\exp(-(\frac{x}{\sigma_x})^2 + (\frac{y}{\sigma_y})^2 + \frac{s^2 + 2ss_0 + s_0^2 + s^2 - 2ss_0 + s_0^2}{2\sigma_z^2})$$\
$$= \frac{1}{(2\pi)^3(\sigma_x\sigma_y\sigma_z)^2}\exp(-(\frac{x}{\sigma_x})^2 + (\frac{y}{\sigma_y})^2 + (\frac{s}{\sigma_z})^2 + (\frac{s_0}{\sigma_z})^2)$$\
$$\Rightarrow \mathcal{L} = 
\frac{2fN_1N_2N_b}{(2\pi)^3(\sigma_x\sigma_y\sigma_z)^2}
\int_{-\infty}^{\infty}\int_{-\infty}^{\infty}\int_{-\infty}^{\infty}\int_{-\infty}^{\infty}
\exp(-(\frac{x}{\sigma_x})^2 + (\frac{y}{\sigma_y})^2 + (\frac{s}{\sigma_z})^2 + (\frac{s_0}{\sigma_z})^2) dx dy ds ds_0$$

Using:\
$$\int_{-\infty}^{\infty}\exp(-ax^2)dx = \sqrt{\frac{\pi}{a}}$$\
We arrive at:\
$$\Rightarrow \mathcal{L}  = \frac{fN_1N_2N_b}{4\pi\sigma_x\sigma_y}$$

## 1b. Luminosity of two different short bunches:
$$\sigma_{x1} \neq \sigma_{x2}$$\
$$\sigma_{y1} \neq \sigma_{y2}$$\
$$\sigma_{z1} = \sigma_{z2} = \sigma_{z}$$

RMS = $$\sqrt{\frac{1}{n}\sum_ix_i^2}$$\
$$\Rightarrow \sigma_i = \sqrt{\frac{1}{2}(\sigma_{i1}^2 + \sigma_{i2}^2)}$$

Then from 1:\
$$\Rightarrow \mathcal{L} = \frac{fN_1N_2N_b}{4\pi\sqrt{\frac{1}{2}(\sigma_{x1}^2 + \sigma_{x2}^2)}\sqrt{\frac{1}{2}(\sigma_{y1}^2 + \sigma_{y2}^2)}}$$
$$= \frac{fN_1N_2N_b}{2\pi\sqrt{\sigma_{x_1}^2 + \sigma_{x_2}^2}\sqrt{\sigma_{y_1}^2 + \sigma_{y_2}^2}}$$

## 2. Crossing Angle For Round Gaussian Beams

The rotation matrices explicitly give the following transformations:

$$ x_1 = x \cos \frac{\phi}{2} - s \sin \frac{\phi}{2}$$\
$$ x_2 = x \cos \frac{\phi}{2} + s \sin \frac{\phi}{2}$$\
$$ s_1 = s \cos \frac{\phi}{2} + x \sin \frac{\phi}{2}$$\
$$ s_2 = s \cos \frac{\phi}{2} - x \sin \frac{\phi}{2}$$

For crossing angle case: $$K = 2\cos^2(\frac{\phi}{2})$$\
$$ \Rightarrow \mathcal{L} = \frac{2\cos^2(\frac{\phi}{2})fN_1N_2N_b}{(2\pi)^3(\sigma_x\sigma_y\sigma_s)^2}\int_{-\infty}^{\infty}\int_{-\infty}^{\infty}\int_{-\infty}^{\infty}\int_{-\infty}^{\infty} 
\exp(-\frac{(x_1^2 + x_2^2)}{2\sigma_x^2})
\exp(-\frac{y^2}{\sigma_y^2})
\exp(-\frac{(s_1 - s_0)^2 + (s_2 + s_0)^2}{2\sigma_s^2}) dx dy ds ds_0$$

Integrate wrt $$y$$:\
$$ \Rightarrow \mathcal{L} = \frac{\cos^2(\frac{\phi}{2})fN_1N_2N_b}{4\pi^{5/2}(\sigma_x\sigma_s)^2\sigma_y}\int_{-\infty}^{\infty}\int_{-\infty}^{\infty}\int_{-\infty}^{\infty} 
\exp(-\frac{(x_1^2 + x_2^2)}{2\sigma_x^2})
\exp(-\frac{(s_1 - s_0)^2 + (s_2 + s_0)^2}{2\sigma_s^2}) dx ds ds_0$$\
$$ \Rightarrow \mathcal{L} = \frac{\cos^2(\frac{\phi}{2})fN_1N_2N_b}{4\pi^{5/2}(\sigma_x\sigma_s)^2\sigma_y}\int_{-\infty}^{\infty}\int_{-\infty}^{\infty}\int_{-\infty}^{\infty} 
\exp(-\frac{(x_1^2 + x_2^2)}{2\sigma_x^2})
\exp(-\frac{s_1^2 + s_2^2 + 2s_0^2 + 2s_0(s_2 - s_1)}{2\sigma_s^2}) dx ds ds_0$$\
Using:\
$$\int_{-\infty}^{\infty}\exp(-(ax^2 + bx + c))dx = \sqrt{\frac{\pi}{a}}\exp(\frac{b^2}{4a} - c)$$\
To integrate over $$s_0$$:\
$$ \Rightarrow \mathcal{L} = \frac{\cos^2(\frac{\phi}{2})fN_1N_2N_b}{4\pi^2\sigma_x^2\sigma_y\sigma_s}\int_{-\infty}^{\infty}\int_{-\infty}^{\infty} 
\exp(-\frac{x_1^2 + x_2^2}{2\sigma_x^2})
\exp(\frac{(s_2 - s_1)^2}{4\sigma_s^2} - \frac{s_1^2 + s_2^2}{2\sigma_s^2}) dx ds$$\
Substitute change of coordinates and simplifying:\
$$ \Rightarrow \mathcal{L} = \frac{\cos^2(\frac{\phi}{2})fN_1N_2N_b}{4\pi^2\sigma_x^2\sigma_y\sigma_s}\int_{-\infty}^{\infty}\int_{-\infty}^{\infty} 
\exp(-\frac{x^2\cos(\frac{\phi}{2})}{\sigma_x^2})
\exp(-s^2(\frac{\sin(\frac{\phi}{2})}{\sigma_x^2} + \frac{\cos(\frac{\phi}{2})}{\sigma_s^2})) dx ds$$\
Integrate wrt $$x$$:\
$$ \Rightarrow \mathcal{L} = \frac{\cos(\frac{\phi}{2})fN_1N_2N_b}{4\pi^{3/2}\sigma_x\sigma_y\sigma_s}\int_{-\infty}^{\infty} 
\exp(-s^2(\frac{\sin(\frac{\phi}{2})}{\sigma_x^2} + \frac{\cos(\frac{\phi}{2})}{\sigma_s^2})) ds$$\
If $$\sigma_x, \sigma_y$$ depend on $$s$$ due to hourglass effect, the expression can no longer be simplified, and $$\sigma_x, \sigma_y$$ go in the $$s$$ integrand.\
Integrate wrt $$s$$ for constant $$\sigma_x, \sigma_y$$:\
$$ \Rightarrow \mathcal{L} = \frac{\cos(\frac{\phi}{2})fN_1N_2N_b}{4\pi\sigma_x\sigma_y\sigma_s}(\frac{\sin(\frac{\phi}{2})}{\sigma_x^2} + \frac{\cos(\frac{\phi}{2})}{\sigma_s^2})^{-\frac12}$$\
Simplifiying further gives:\
$$ \Rightarrow \mathcal{L} = \frac{fN_1N_2N_b}{4\pi\sigma_x\sigma_y}\frac{1}{\sqrt{1 + (\frac{\sigma_s}{\sigma_x})^2\tan^2(\frac{\phi}{2})}}$$\
Finally:\
$$ \mathcal{L_{CA}} = L_0 S(\phi)$$




Sources: 
[https://cds.cern.ch/record/941318/files/p361.pdf](https://cds.cern.ch/record/941318/files/p361.pdf)